Alphas added.

TrLowLevel.v
@@ -22,63 +22,74 @@ Require Export Semantics.
 
 (* ---------------------------------------------------------------------- *)
 
+Definition in_block (m:state) (l1:loc) (l:loc) : Prop :=
+  exists ws,
+      m[l1] = val_words ws
+  /\  l1 <= l < l1 + length ws.
+
+Definition disjoint_blocks (m:state) : Prop :=
+  forall l1 l2,
+    l1 <> l2 ->
+    forall l, ~ (in_block m l1 l /\ in_block m l1 l).
+
 (** Transformation of states: m ~ |m| *)
 
-Inductive tr_state (C:typdefctx) (LLC:ll_typdefctx) (φ:phi) : state -> state -> Prop :=
+Inductive tr_state (C:typdefctx) (LLC:ll_typdefctx) (φ:phi) (α:alpha) : state -> state -> Prop :=
   | tr_state_intro : forall m m',
       dom m = dom m' ->
+      disjoint_blocks m' ->
       (forall l lw T,
         l \indom m ->
             typing_val C LLC φ m[l] T
-        /\  tr_ll_val C LLC T m[l] lw
-        /\  m'[l] = val_words lw) ->
-      tr_state C LLC φ m m'.
+        /\  tr_ll_val C LLC α T m[l] lw
+        /\  m'[α[l]] = val_words lw) ->
+      tr_state C LLC φ α m m'.
 
 (* ---------------------------------------------------------------------- *)
 (* Transformation of a term from high-level to low-level. This is how the code is transformed. *)
 
-Inductive tr_val (C:typdefctx) (LLC:ll_typdefctx) : val -> val -> Prop :=
+Inductive tr_val (C:typdefctx) (LLC:ll_typdefctx) (α:alpha) : val -> val -> Prop :=
   | tr_val_error :
-      tr_val C LLC val_error val_error
+      tr_val C LLC α val_error val_error
   | tr_val_unit :
-      tr_val C LLC val_unit val_unit
+      tr_val C LLC α val_unit val_unit
   | tr_val_bool : forall b,
-      tr_val C LLC (val_bool b) (val_bool b)
+      tr_val C LLC α (val_bool b) (val_bool b)
   | tr_val_int : forall i,
-      tr_val C LLC (val_int i) (val_int i)
+      tr_val C LLC α (val_int i) (val_int i)
   | tr_val_double : forall d,
-      tr_val C LLC (val_double d) (val_double d)
+      tr_val C LLC α (val_double d) (val_double d)
   | tr_val_abstract_ptr : forall π l o,
       tr_ll_accesses C LLC π o ->
-      tr_val C LLC (val_abstract_ptr l π) (val_concrete_ptr l o)
+      tr_val C LLC α (val_abstract_ptr l π) (val_concrete_ptr α[l] o)
   | tr_val_array : forall T a a',
-      List.Forall2 (tr_val C LLC) a a' ->
-      tr_val C LLC (val_array T a) (val_array T a')
+      List.Forall2 (tr_val C LLC α) a a' ->
+      tr_val C LLC α (val_array T a) (val_array T a')
   | tr_val_struct : forall Tv s s',
       dom s = dom s' ->
       (forall f,
         index s f ->
-        tr_val C LLC s[f] s'[f]) ->
-      tr_val C LLC (val_struct (typ_var Tv) s) (val_struct (typ_var Tv) s').
+        tr_val C LLC α s[f] s'[f]) ->
+      tr_val C LLC α (val_struct (typ_var Tv) s) (val_struct (typ_var Tv) s').
 
 (** Transformation of stacks: S ~ |S| *)
 
-Inductive tr_stack_item (C:typdefctx) (LLC:ll_typdefctx) : (var * val) -> (var * val) -> Prop :=
+Inductive tr_stack_item (C:typdefctx) (LLC:ll_typdefctx) (α:alpha) : (var * val) -> (var * val) -> Prop :=
   | tr_stack_item_intro : forall x v v',
-      tr_val C LLC v v' -> 
-      tr_stack_item C LLC (x, v) (x, v').
+      tr_val C LLC α v v' -> 
+      tr_stack_item C LLC α (x, v) (x, v').
 
-Inductive tr_stack (C:typdefctx) (LLC:ll_typdefctx) : stack -> stack -> Prop :=
+Inductive tr_stack (C:typdefctx) (LLC:ll_typdefctx) (α:alpha) : stack -> stack -> Prop :=
   | tr_stack_intro : forall S S',
-      LibList.Forall2 (tr_stack_item C LLC) S S' ->
-      tr_stack C LLC S S'.
+      LibList.Forall2 (tr_stack_item C LLC α) S S' ->
+      tr_stack C LLC α S S'.
 
-Lemma stack_lookup_tr : forall C LLC S S' x v,
-  tr_stack C LLC S S' ->
+Lemma stack_lookup_tr : forall C LLC α S S' x v,
+  tr_stack C LLC α S S' ->
   Ctx.lookup x S = Some v -> 
     exists v', 
        Ctx.lookup x S' = Some v' 
-    /\ tr_val C LLC v v'.
+    /\ tr_val C LLC α v v'.
 Proof.
   introv HS Hx. inverts HS as HS. induction HS.
   { inverts Hx. }
@@ -90,33 +101,33 @@ Qed.
 
 (** Transformation of terms: t ~ |t| *)
 
-Inductive tr_trm (C:typdefctx) (LLC:ll_typdefctx) : trm -> trm -> Prop :=
+Inductive tr_trm (C:typdefctx) (LLC:ll_typdefctx) (α:alpha) : trm -> trm -> Prop :=
   | tr_trm_val : forall v v',
-      tr_val C LLC v v' ->
-      tr_trm C LLC (trm_val v) (trm_val v')
+      tr_val C LLC α v v' ->
+      tr_trm C LLC α (trm_val v) (trm_val v')
   | tr_trm_var : forall x,
-      tr_trm C LLC (trm_var x) (trm_var x)
+      tr_trm C LLC α (trm_var x) (trm_var x)
   | tr_trm_if : forall t0 t1 t2 t0' t1' t2',
-      tr_trm C LLC t0 t0' ->
-      tr_trm C LLC t1 t1' ->
-      tr_trm C LLC t2 t2' ->
-      tr_trm C LLC (trm_if t0 t1 t2) (trm_if t0' t1' t2')
+      tr_trm C LLC α t0 t0' ->
+      tr_trm C LLC α t1 t1' ->
+      tr_trm C LLC α t2 t2' ->
+      tr_trm C LLC α (trm_if t0 t1 t2) (trm_if t0' t1' t2')
   | tr_trm_let : forall t0 t1 z t0' t1',
-      tr_trm C LLC t0 t0' ->
-      tr_trm C LLC t1 t1' ->
-      tr_trm C LLC (trm_let z t0 t1) (trm_let z t0' t1')
+      tr_trm C LLC α t0 t0' ->
+      tr_trm C LLC α t1 t1' ->
+      tr_trm C LLC α (trm_let z t0 t1) (trm_let z t0' t1')
   | tr_trm_binop : forall t1 t2 op t1' t2', 
-      tr_trm C LLC t1 t1' ->
-      tr_trm C LLC t2 t2' ->
-      tr_trm C LLC (trm_app (prim_binop op) (t1::t2::nil)) (trm_app (prim_binop op) (t1'::t2'::nil))
+      tr_trm C LLC α t1 t1' ->
+      tr_trm C LLC α t2 t2' ->
+      tr_trm C LLC α (trm_app (prim_binop op) (t1::t2::nil)) (trm_app (prim_binop op) (t1'::t2'::nil))
   | tr_trm_get : forall t1 T t1',
-      tr_trm C LLC t1 t1' ->
-      tr_trm C LLC (trm_app (prim_get T) (t1::nil)) (trm_app (prim_ll_get T) (t1'::nil))
+      tr_trm C LLC α t1 t1' ->
+      tr_trm C LLC α (trm_app (prim_get T) (t1::nil)) (trm_app (prim_ll_get T) (t1'::nil))
   | tr_trm_set : forall t1 t2 T t1' t2',
-      tr_trm C LLC t1 t1' ->
-      tr_trm C LLC (trm_app (prim_set T) (t1::t2::nil)) (trm_app (prim_ll_set T) (t1'::t2'::nil))
+      tr_trm C LLC α t1 t1' ->
+      tr_trm C LLC α (trm_app (prim_set T) (t1::t2::nil)) (trm_app (prim_ll_set T) (t1'::t2'::nil))
   | tr_trm_new : forall T,
-      tr_trm C LLC (trm_app (prim_new T) nil) (trm_app (prim_ll_new T) nil)
+      tr_trm C LLC α (trm_app (prim_new T) nil) (trm_app (prim_ll_new T) nil)
  (*| tr_trm_new_array :
       TODO: prim_new_array is needed here. *)
   | tr_trm_struct_access : forall Tfs t1' o Tv f t1 tr,
@@ -124,24 +135,24 @@ Inductive tr_trm (C:typdefctx) (LLC:ll_typdefctx) : trm -> trm -> Prop :=
       typing_struct C (typ_var Tv) Tfs ->
       f \indom Tfs ->
       o = (fields_offsets LLC)[Tv][f] ->
-      tr_trm C LLC t1 t1' ->
+      tr_trm C LLC α t1 t1' ->
       tr = trm_app (prim_ll_access Tfs[f]) (t1'::(trm_val (val_int o))::nil) ->
-      tr_trm C LLC (trm_app (prim_struct_access (typ_var Tv) f) (t1::nil)) tr
+      tr_trm C LLC α (trm_app (prim_struct_access (typ_var Tv) f) (t1::nil)) tr
   | tr_trm_array_access : forall os t2' n tr T' t1' toff T t1 t2,
       typing_array C T T' os ->
       typ_size (typvar_sizes LLC) T' n ->
-      tr_trm C LLC t1 t1' ->
-      tr_trm C LLC t2 t2' ->
+      tr_trm C LLC α t1 t1' ->
+      tr_trm C LLC α t2 t2' ->
       toff = trm_app (prim_binop binop_mul) (t2'::(trm_val (val_int n))::nil) ->
       tr = trm_app (prim_ll_access T') (t1'::toff::nil) ->
-      tr_trm C LLC (trm_app (prim_array_access T) (t1::t2::nil)) tr
+      tr_trm C LLC α (trm_app (prim_array_access T) (t1::t2::nil)) tr
   | tr_trm_struct_get : forall t1 T f t1',
-      tr_trm C LLC t1 t1' ->
-      tr_trm C LLC (trm_app (prim_struct_get T f) (t1::nil)) (trm_app (prim_struct_get T f) (t1'::nil))
+      tr_trm C LLC α t1 t1' ->
+      tr_trm C LLC α (trm_app (prim_struct_get T f) (t1::nil)) (trm_app (prim_struct_get T f) (t1'::nil))
   | tr_trm_array_get : forall t1 t2 T t1' t2',
-      tr_trm C LLC t1 t1' ->
-      tr_trm C LLC t2 t2' ->
-      tr_trm C LLC (trm_app (prim_array_get T) (t1::t2::nil)) (trm_app (prim_array_get T) (t1'::t2'::nil)).
+      tr_trm C LLC α t1 t1' ->
+      tr_trm C LLC α t2 t2' ->
+      tr_trm C LLC α (trm_app (prim_array_get T) (t1::t2::nil)) (trm_app (prim_array_get T) (t1'::t2'::nil)).
 
 (* ---------------------------------------------------------------------- *)
 (** Correctness of the transformation *)
